Test/generated/smt/case_if_constr.smt2
@@ -149,5 +149,5 @@
 (declare-fun uplc_g2_multiScalarMul (ValList ValList) G2)
 (declare-const $u$120 Int)
 (assert (let ((|moist.dag.0| (= $u$120 10))) (or (and |moist.dag.0| (= 1 1)) (and (not |moist.dag.0|) (= 0 1)))))
-(check-sat)
+(check-sat-using (then simplify ctx-solver-simplify smt))
 (get-model)
